# Stirling Numbers 

Tristan Chaang

March 11, 2022

In this article we will look at Stirling Numbers.

## Contents

1 First Kind ..... 1
2 Second Kind ..... 2
3 Examples ..... 3
4 Finite Difference and Finite Integration ..... 4

## 1 First Kind

Consider the group $S_{n}$ of permutations of $[n]=\{1, \cdots, n\}$. Any permutation $\sigma \in S_{n}$ can be uniquely decomposed into disjoint cycles, for example the permutation $(1,2,3,4,5) \mapsto(2,5,4,3,1)$ can be written as (125)(34). This permutation has 2 cycles.

Definition. The number of permutations in $S_{n}$ with $k$ cycles is denoted by $c(n, k)$.

For any positive $n$,

- $c(n, n)=1$ because the only permutation with $n$ cycles is $(1)(2) \cdots(n)$.
- $c(n, 1)=(n-1)$ ! because there are $n!/ n$ cyclic permutations of $[n]$.
- $c(n, k)=0$ for $k \leq 0$ or $k>n$.

Proposition 1.1. For any integers $n, k, c(n, k)=c(n-1, k-1)+(n-1) \cdot c(n-1, k)$.
Proof. For any permutation of [ $n$ ] with $k$ cycles, the cycle that contains $n$ can contain one element (only $n$ ), or more than one element. In the former case, those permutations have a one-to-one correspondence with permutations of $[n-1]$ with $k-1$ cycles. In the latter case, those permutations have a one-to- $(n-1)$ correspondence with permutations $\sigma^{\prime}$ of $[n-1]$ with $k$ cycles because $n$ can be slotted anywhere in the cyclic decomposition of $\sigma^{\prime}$.

Proposition 1.2. $x(x+1) \cdots(x+n-1)=\sum_{k} c(n, k) x^{k}$.

Proof. Let $x(x+1) \cdots(x+n-1)=\sum_{k} c_{0}(n, k) x^{k}$. Obviously $c_{0}(1, k)=c(1, k)$. By induction, it remains to verify the recursive property:

$$
\begin{aligned}
\sum_{k} c_{0}(n, k) x^{k} & =x(x+1) \cdots(x+n-1) \\
& =(x+n-1) \sum_{k} c_{0}(n-1, k) x^{k} \\
& =\sum_{k}(c(n-1, k-1)+(n-1) \cdot c(n-1, k)) x^{k}
\end{aligned}
$$

Proposition 1.3. $x(x-1) \cdots(x-n+1)=\sum_{k}(-1)^{n+k} c(n, k) x^{k}$.
Proof. Using proposition 2,

$$
\begin{aligned}
x(x-1) \cdots(x-n+1) & =(-1)^{n}(-x)(-x+1) \cdots(-x+n-1) \\
& =(-1)^{n} \sum_{k} c(n, k)(-x)^{k} \\
& =\sum_{k}(-1)^{n+k} c(n, k) x^{k} .
\end{aligned}
$$

Definition. The numbers $\left[\begin{array}{l}n \\ k\end{array}\right]=(-1)^{n+k} c(n, k)$ are called Stirling Numbers of the First Kind.
Define $x^{(n)}=x(x-1) \cdots(x-n+1)$. From proposition 3,

$$
x^{(n)}=\sum_{k}\left[\begin{array}{l}
n \\
k
\end{array}\right] x^{k} .
$$

## 2 Second Kind

A set partition of $[n]$ is a collection of a disjoint subsets of $[n]$ whose union is $[n]$. For example,

$$
\{\{1,2,3\},\{4,6\},\{5\}\}
$$

is a set partition of $[6]=\{1,2,3,4,5,6\}$, with 3 parts.
Definition. The number of set partitions of [n] with $k$ parts is denoted by $\left\{\begin{array}{l}n \\ k\end{array}\right\}$. These numbers are called Stirling Numbers of the Second Kind.

For any positive $n$,

- $\left\{\begin{array}{l}n \\ 1\end{array}\right\}=1$ because the only set partition with 1 part is $\{\{1, \cdots, n\}\}$.
- $\left\{\begin{array}{l}n \\ n\end{array}\right\}=1$ because the only set partition with 1 part is $\{\{1\}, \cdots,\{n\}\}$.
- $\left\{\begin{array}{l}n \\ k\end{array}\right\}=0$ for $k \leq 0$ or $k>n$.

Proposition 2.1. For any integers $n, k,\left\{\begin{array}{l}n \\ k\end{array}\right\}=\left\{\begin{array}{l}n-1 \\ k-1\end{array}\right\}+k\left\{\begin{array}{c}n-1 \\ k\end{array}\right\}$.
Proof. For any set partition of $[n]$ with $k$ parts, the part that contains $n$ can contain one element (i.e. $\{n\}$ ), or more than one element. In the former case, those partitions have a one-to-one correspondence with set partitions of $[n-1]$ with $k-1$ parts. In the latter case, those partitions have a one-to- $k$ correspondence with set partitions $\sigma^{\prime}$ of $[n-1]$ with $k$ parts because $n$ can be in any of the $k$ parts of $\sigma^{\prime}$.

Proposition 2.2. $x^{n}=\sum_{k}\left\{\begin{array}{l}n \\ k\end{array}\right\} x^{(k)}$.
Proof. For $n=1$ it is true. Now,

$$
\begin{aligned}
\sum_{k}\left\{\begin{array}{l}
n \\
k
\end{array}\right\} x^{(k)} & =x^{n}=x \sum_{k}\left\{\begin{array}{c}
n-1 \\
k
\end{array}\right\} x^{(k)} \\
& =\sum_{k}\left\{\begin{array}{c}
n-1 \\
k
\end{array}\right\}(x-k+k) x^{(k)} \\
& =\sum_{k}\left(k\left\{\begin{array}{c}
n-1 \\
k
\end{array}\right\}+\left\{\begin{array}{l}
n-1 \\
k-1
\end{array}\right\}\right) x^{(k)}
\end{aligned}
$$

so by induction it is true for all $n$.
Proposition 2.3. If $S$ and $s$ are infinite matrices where $S_{i j}=\left[\begin{array}{l}i \\ j\end{array}\right]$ and $s_{i j}=\left\{\begin{array}{l}i \\ j\end{array}\right\}$, then $S s=I$.
Proof. Since $\left\{x^{n}\right\}$ and $\left\{x^{(n)}\right\}$ are bases for the vector space $\mathbb{R}[x]$, proposition 1.3 and 2.2 shows that $S$ and $s$ are just matrices of basis change between $\left\{x^{n}\right\}$ and $\left\{x^{(n)}\right\}$, so they are inverses of each other.

## 3 Examples

Example 1. Find $\left[\begin{array}{c}n+1 \\ n\end{array}\right]$.
Solution. $\left[\begin{array}{c}n+1 \\ n\end{array}\right]=\left[\begin{array}{c}n \\ n-1\end{array}\right]+n\left[\begin{array}{l}n \\ n\end{array}\right]=\left[\begin{array}{c}n \\ n-1\end{array}\right]+n$, so

$$
\left[\begin{array}{c}
n+1 \\
n
\end{array}\right]=n+(n-1)+\cdots+1=\frac{n(n+1)}{2}
$$

Example 2. Find $\left[\begin{array}{c}n+2 \\ n\end{array}\right]$.
Solution. $\left[\begin{array}{c}n+2 \\ n\end{array}\right]=\left[\begin{array}{l}n+1 \\ n-1\end{array}\right]+(n+1)\left[\begin{array}{c}n+1 \\ n\end{array}\right]=\left[\begin{array}{c}n+1 \\ n-1\end{array}\right]+\frac{n(n+1)^{2}}{2}$, so

$$
\left[\begin{array}{c}
n+2 \\
n
\end{array}\right]=\sum_{k=1}^{n} \frac{k(k+1)^{2}}{2}=\frac{n(n+1)(n+2)(3 n+5)}{24}
$$

Example 3. Find $\left\{\begin{array}{c}n+1 \\ n\end{array}\right\}$.

Solution. $\left\{\begin{array}{c}n+1 \\ n\end{array}\right\}=\left\{\begin{array}{c}n \\ n-1\end{array}\right\}+n\left\{\begin{array}{l}n \\ n\end{array}\right\}=\left\{\begin{array}{c}n \\ n-1\end{array}\right\}+n$, so

$$
\left\{\begin{array}{c}
n+1 \\
n
\end{array}\right\}=n+(n-1)+\cdots+1=\frac{n(n+1)}{2}
$$

Example 3. Find $\left\{\begin{array}{c}n+2 \\ n\end{array}\right\}$.
Solution. $\left\{\begin{array}{c}n+2 \\ n\end{array}\right\}=\left\{\begin{array}{c}n+1 \\ n-1\end{array}\right\}+n\left\{\begin{array}{c}n+1 \\ n\end{array}\right\}=\left\{\begin{array}{c}n \\ n-1\end{array}\right\}+\frac{n^{2}(n+1)}{2}$, so

$$
\left\{\begin{array}{c}
n+2 \\
n
\end{array}\right\}=\sum_{k=1}^{n} \frac{k^{2}(k+1)}{2}=\frac{n(n+1)(n+2)(3 n+1)}{24}
$$

Example 4. Find $\left\{\begin{array}{c}n+3 \\ n\end{array}\right\}$.
Solution. $\left\{\begin{array}{c}n+3 \\ n\end{array}\right\}=\left\{\begin{array}{c}n+2 \\ n-1\end{array}\right\}+n\left\{\begin{array}{c}n+2 \\ n\end{array}\right\}=\left\{\begin{array}{c}n \\ n-1\end{array}\right\}+\frac{n^{2}(n+1)(n+2)(3 n+1)}{24}$, so

$$
\left\{\begin{array}{c}
n+1 \\
n
\end{array}\right\}=\sum_{k=1}^{n} \frac{k^{2}(k+1)(k+2)(3 k+1)}{24}=\frac{n^{2}(n+1)^{2}(n+2)(n+3)}{48}
$$

## 4 Finite Difference and Finite Integration

This section requires knowledge from my previous article, Finite Differences.
Example 1. Find the value of $\sum_{k=0}^{n}(-1)^{k}\binom{n}{k} k^{n+1}$.
Solution. We basically want $(I-E)^{n} x^{n+1}=(-1)^{n} \Delta^{n} x^{n+1}$ evaluated at $x=0$.

$$
\begin{aligned}
\Delta^{n}\left(x^{n+1}\right) & =\Delta^{n}\left(x^{(n+1)}+\left\{\begin{array}{c}
n+1 \\
n
\end{array}\right\} x^{(n)}+\cdots\right) \\
& =(n+1)^{(n)} x^{(1)}+n!\left\{\begin{array}{c}
n+1 \\
n
\end{array}\right\},
\end{aligned}
$$

so the answer is

$$
(-1)^{n} n!\left\{\begin{array}{c}
n+1 \\
n
\end{array}\right\}=(-1)^{n} n!\cdot \frac{n(n+1)}{2}=(-1)^{n} \cdot \frac{(n+1)!n}{2}
$$

Example 2. Find the value of $\sum_{k=0}^{n}(-1)^{k}\binom{n}{k} k^{n+2}$.
Solution. We basically want $(I-E)^{n} x^{n+2}=(-1)^{n} \Delta^{n} x^{n+2}$ evaluated at $x=0$.

$$
\begin{aligned}
\Delta^{n}\left(x^{n+2}\right) & =\Delta^{n}\left(x^{(n+2)}+\left\{\begin{array}{l}
n+2 \\
n+1
\end{array}\right\} x^{(n+1)}+\left\{\begin{array}{c}
n+2 \\
n
\end{array}\right\} x^{(n)}+\cdots\right) \\
& =(n+2)^{(n)} x^{(2)}+(n+1)^{(n)}\left\{\begin{array}{l}
n+2 \\
n+1
\end{array}\right\} x^{(1)}+n!\left\{\begin{array}{c}
n+2 \\
n
\end{array}\right\}
\end{aligned}
$$

so the answer is

$$
(-1)^{n} n!\left\{\begin{array}{c}
n+2 \\
n
\end{array}\right\}=(-1)^{n} n!\cdot \frac{n(n+1)(n+2)(3 n+1)}{24}=(-1)^{n} \cdot \frac{(n+2)!(3 n+1) n}{24}
$$

Example 3. Find the value of $\sum_{k=0}^{n}(-1)^{k}\binom{n}{k} k^{n+3}$.
Solution. We basically want $(I-E)^{n} x^{n+3}=(-1)^{n} \Delta^{n} x^{n+3}$ evaluated at $x=0$.

$$
\begin{aligned}
\Delta^{n}\left(x^{n+3}\right) & =\Delta^{n}\left(x^{(n+3)}+\left\{\begin{array}{l}
n+3 \\
n+2
\end{array}\right\} x^{(n+2)}+\left\{\begin{array}{l}
n+3 \\
n+1
\end{array}\right\} x^{(n+1)}+\left\{\begin{array}{c}
n+3 \\
n
\end{array}\right\} x^{(n)}+\cdots\right) \\
& =(n+3)^{(n)} x^{(3)}+(n+2)^{(n)}\left\{\begin{array}{l}
n+3 \\
n+2
\end{array}\right\} x^{(2)}+(n+1)^{(n)}\left\{\begin{array}{c}
n+3 \\
n+1
\end{array}\right\} x^{(1)}+n!\left\{\begin{array}{c}
n+3 \\
n
\end{array}\right\},
\end{aligned}
$$

so the answer is

$$
(-1)^{n} n!\left\{\begin{array}{c}
n+3 \\
n
\end{array}\right\}=(-1)^{n} n!\cdot \frac{n^{2}(n+1)^{2}(n+2)(n+3)}{48}=(-1)^{n} \cdot \frac{(n+2)!(n+1)(n+3) n^{2}}{24}
$$

## References

[1] Stirling Numbers of the First Kind
https://en.wikipedia.org/wiki/Stirling_numbers_of_the_first_kind
[2] Stirling Numbers of the Second Kind
https://en.wikipedia.org/wiki/Stirling_numbers_of_the_second_kind
[3] Finite Differences
https://tristanchaang.github.io/2022/01/22/finite-differences.html

